Moved all mapping-related results into one file.

HOL/DataStrs/Mapping.thy
@@ -1,5 +1,5 @@
 theory Mapping
-imports "../Logic_More"
+imports "../Auto2_Main"
 begin
 
 datatype ('a, 'b) map = Map "'a \<Rightarrow> 'b option"
@@ -38,5 +38,123 @@ setup {* del_prfstep_thm @{thm map_of_alist_def} *}
 theorem map_of_alist_nil [rewrite]:
   "x \<notin> set (map fst ys) \<Longrightarrow> (map_of_alist ys)\<langle>x\<rangle> = None"
 @proof @induct ys @qed
+
+section {* The unique *}
+
+definition THE_unique :: "('a \<Rightarrow> bool) \<Rightarrow> 'a option" where
+  "THE_unique P = (if (\<exists>!x. P x) then Some (THE x. P x) else None)"
+setup {* add_rewrite_rule @{thm THE_unique_def} *}
+
+theorem THE_uniqueI: "\<exists>!x. P x \<Longrightarrow> THE_unique P \<noteq> None \<and> P (the (THE_unique P))" by auto2
+setup {* add_forward_prfstep_cond @{thm THE_uniqueI} [with_term "THE_unique ?P"] *}
+
+theorem THE_unique_None: "\<not>(\<exists>!x. P x) \<Longrightarrow> THE_unique P = None" by auto2
+setup {* add_forward_prfstep_cond @{thm THE_unique_None} [with_term "THE_unique ?P"] *}
+
+theorem THE_unique_None': "\<not>(\<exists>x. P x) \<Longrightarrow> THE_unique P = None" by auto2
+setup {* add_forward_prfstep_cond @{thm THE_unique_None'} [with_term "THE_unique ?P"] *}
+
+theorem THE_unique_eq: "P a \<Longrightarrow> \<exists>!x. P x \<Longrightarrow> THE_unique P = Some a" by auto2
+setup {* add_forward_prfstep_cond @{thm THE_unique_eq} [with_term "THE_unique ?P"] *}
+
+theorem THE_uniqueD [resolve]: "THE_unique P = Some x \<Longrightarrow> P x"
+  by (metis THE_unique_def option.sel option.simps(3) theI')
+
+setup {* del_prfstep_thm @{thm THE_unique_def} *}
+    
+section {* Unique keys in an alist *}
+
+definition unique_keys :: "(nat \<times> 'a) list \<Rightarrow> bool" where [rewrite]:
+  "unique_keys xs = (\<forall>m n. m < length xs \<longrightarrow> n < length xs \<longrightarrow> m \<noteq> n \<longrightarrow> fst (xs ! m) \<noteq> fst (xs ! n))"
+setup {* add_property_const @{term unique_keys} *}
+
+lemma unique_keysD:
+  "unique_keys xs \<Longrightarrow> m < length xs \<Longrightarrow> n < length xs \<Longrightarrow> m \<noteq> n \<Longrightarrow> fst (xs ! m) \<noteq> fst (xs ! n)" by auto2
+setup {* add_forward_prfstep_cond @{thm unique_keysD} [with_term "?xs ! ?m", with_term "?xs ! ?n"] *}
+setup {* del_prfstep_thm_eqforward @{thm unique_keys_def} *}
+
+definition has_key :: "(nat \<times> 'a) list \<Rightarrow> nat \<Rightarrow> bool" where
+  "has_key xs k = (\<exists>v'. (k, v') \<in># mset xs)"
+setup {* add_rewrite_rule @{thm has_key_def} *}
+
+theorem not_has_key [forward, backward2]:
+  "\<not>(has_key xs k) \<Longrightarrow> p \<in># mset xs \<Longrightarrow> k \<noteq> fst p" by auto2
+
+definition map_of_kv_set :: "('a \<times> 'b) set \<Rightarrow> ('a, 'b) map" where
+  "map_of_kv_set S = Map (\<lambda>a. THE_unique (\<lambda>b. (a, b) \<in> S))"
+setup {* add_rewrite_rule @{thm map_of_kv_set_def} *}
+
+setup {* add_gen_prfstep ("THE_unique_case",
+  [WithTerm @{term_pat "THE_unique (\<lambda>b. (?a, b) \<in> ?S)"},
+   CreateCase @{term_pat "\<exists>!b. (?a, b) \<in> ?S"}]) *}
+
+definition unique_keys_set :: "(nat \<times> 'a) set \<Rightarrow> bool" where
+  "unique_keys_set S = (\<forall>i x y. (i, x) \<in> S \<longrightarrow> (i, y) \<in> S \<longrightarrow> x = y)"
+setup {* add_rewrite_rule @{thm unique_keys_set_def} *}
+
+theorem unique_keys_imp [forward]:
+  "unique_keys_set S \<Longrightarrow> (i, x) \<in> S \<Longrightarrow> \<exists>!x. (i, x) \<in> S" by auto2
+
+theorem in_set_union_single: "x \<in> A \<union> {y} \<Longrightarrow> x = y \<or> x \<in> A" by auto
+setup {* add_forward_prfstep_cond @{thm in_set_union_single} [with_cond "?x \<noteq> ?y"] *}
+theorem member_union_single: "x \<in> A \<union> {x}" by simp
+setup {* add_forward_prfstep_cond @{thm member_union_single} [with_term "?A \<union> {?x}"] *}
+
+theorem map_of_kv_set_insert [rewrite]:
+  "unique_keys_set T \<Longrightarrow> \<forall>v. (k, v) \<notin> T \<Longrightarrow> map_of_kv_set (T \<union> { (k, v) }) = (map_of_kv_set T) {k \<rightarrow> v}"
+@proof
+  @let "S = T \<union> { (k, v) }" @then
+  @have "T \<subseteq> S" @then @have "unique_keys_set S"
+@qed
+
+theorem map_of_kv_set_delete [rewrite]:
+  "unique_keys_set T \<Longrightarrow> (k, v) \<in> T \<Longrightarrow> map_of_kv_set (T - { (k, v) }) = delete_map k (map_of_kv_set T)"
+@proof
+  @let "S = T - { (k, v) }" @then
+  @have "S \<subseteq> T" @then @have "unique_keys_set S"
+@qed
+
+theorem map_of_kv_set_update [rewrite]:
+  "unique_keys_set T \<Longrightarrow> (k, v) \<in> T \<Longrightarrow>
+   map_of_kv_set ((T - { (k, v) }) \<union> { (k, v') }) = (map_of_kv_set T) {k \<rightarrow> v'}"
+@proof
+  @have "unique_keys_set (T - { (k, v) })" @then
+  @have "\<forall>x. (k, x) \<notin> T - { (k, v) }"
+@qed
+
+setup {* fold del_prfstep_thm [@{thm in_set_union_single}, @{thm member_union_single}] *}
+
+definition map_of_kv_list :: "('a \<times> 'b) list \<Rightarrow> ('a, 'b) map" where
+  "map_of_kv_list xs = map_of_kv_set (set xs)"
+setup {* add_rewrite_rule @{thm map_of_kv_list_def} *}
+
+setup {* add_forward_prfstep_cond @{thm in_set_conv_nth'} [with_cond "?x \<noteq> ?xs ! ?i"] *}
+theorem unique_keys_to_set [forward]: "unique_keys xs \<Longrightarrow> unique_keys_set (set xs)" by auto2
+setup {* del_prfstep_thm_str "" @{thm in_set_conv_nth'} *}
+
+theorem unique_key_to_distinct [forward]: "unique_keys xs \<Longrightarrow> distinct xs"
+  using distinct_conv_nth unique_keys_def by fastforce
+
+lemma map_of_kv_list_empty [backward]:
+  "[] = xs \<Longrightarrow> map_of_kv_list xs = empty_map" by auto2
+
+theorem mset_update' [rewrite]:
+  "i < length ls \<Longrightarrow> mset (list_update ls i v) = {#v#} + (mset ls - {# ls ! i #})"
+  using mset_update by fastforce
+
+theorem empty_list_to_empty_map [rewrite]:
+  "map_of_kv_list ([]::('a \<times> 'b) list) = empty_map" by auto2
+
+theorem has_key_set [rewrite]:
+  "has_key xs k \<longleftrightarrow> (\<exists>v. (k, v) \<in> set xs)"
+@proof
+  @case "has_key xs k" @with
+    @obtain v where "(k, v) \<in># mset xs" @then @have "(k, v) \<in> set xs"
+  @end
+@qed
+
+theorem has_key_to_map_none [rewrite_bidir]:
+  "unique_keys xs \<Longrightarrow> has_key xs k \<longleftrightarrow> (map_of_kv_list xs) \<langle>k\<rangle> \<noteq> None" by auto2
+setup {* del_prfstep_thm @{thm has_key_set} *}
 
 end
